\section{Details of proofs}

% FIXME: give the explicit equational rules for the type equality

% FIXME: make this look better
\begin{lemma}[\lemref{lem:tyeqsubst-erasure}]
  \begin{enumerate}
  \item If $\Delta \vdash A \equiv B \isType$ then $\tySem{A} =
    \tySem{B}$; and
  \item If $\Delta \vdash A \isType$ and $\sigma : \Delta' \Rightarrow
    \Delta$, then $\tySem{\sigma^*A} = \tySem{A}$.
  \end{enumerate}
\end{lemma}
\begin{proof}
  \begin{enumerate}
  \item By induction on the derivation of $\Delta \vdash A \equiv B
    \isType$:
    \begin{description}
    \item[Case \TirName{TyEqUnit}] In this case, $A = B = \tyUnit$, so
      $\tySem{A} = \tySem{B}$.
    \item[Case \TirName{TyEqPrim}] We have $A =
      \tyPrim{X}{e_1,...,e_n}$ and $B =
      \tyPrim{X}{e'_1,...,e'_n}$. The erasure semantics ignores the
      index arguments, so $\tySem{A} = \tySem{\tyPrim{X}{e_1,...,e_n}}
      = \tyPrimSem{X} = \tySem{\tyPrim{X}{e'_1,...,e'_n}} =
      \tySem{B}$, as required.
    \item[Case \TirName{TyEqArr}] Here, $A = A_1 \tyArr A_2$ and $B =
      B_1 \tyArr B_2$, and by the induction hypothesis we know that
      $\tySem{A_1} = \tySem{B_1}$ and $\tySem{A_2} =
      \tySem{B_2}$. Hence $\tySem{A} = \tySem{A_1 \tyArr A_2} =
      \tySem{A_1} \to \tySem{A_2} = \tySem{B_1} \to \tySem{B_2} =
      \tySem{B_1 \tyArr B_2} = \tySem{B}$.
    \item[Case \TirName{TyEqProd}] In this case, $A = A_1 \tyProduct
      A_2$ and $B = B_1 \tyProduct B_2$, and by the induction
      hypothesis we know that $\tySem{A_1} = \tySem{B_1}$ and
      $\tySem{A_2} = \tySem{B_2}$. Hence $\tySem{A} = \tySem{A_1
        \tyProduct A_2} = \tySem{A_1} \times \tySem{A_2} = \tySem{B_1}
      \times \tySem{B_2} = \tySem{B_1 \tyProduct B_2} = \tySem{B}$.
    \item[Case \TirName{TyEqSum}] In this case, $A = A_1 + A_2$ and $B
      = B_1 + B_2$, and by the induction hypothesis we know that
      $\tySem{A_1} = \tySem{B_1}$ and $\tySem{A_2} =
      \tySem{B_2}$. Hence $\tySem{A} = \tySem{A_1 + A_2} = \tySem{A_1}
      + \tySem{A_2} = \tySem{B_1} + \tySem{B_2} = \tySem{B_1 + B_2} =
      \tySem{B}$.
    \item[Case \TirName{TyEqForall}] We have $A = \forall
      i\mathord:s.A'$ and $B = \forall i\mathord:s.B'$. By the
      induction hypothesis we know that $\tySem{A'} = \tySem{B'}$, and
      hence $\tySem{A} = \tySem{\forall i\mathord:s. A'} = \tySem{A'}
      = \tySem{B'} = \tySem{\forall i\mathord:s. B'} = \tySem{B}$.
    \end{description}
  \item By induction on the derivation of $\Delta \vdash A \isType$.
    \begin{description}
    \item[Case \TirName{TyUnit}] Directly from the definition of
      substitution on types of the form $\tyUnit$, we have
      $\tySem{\sigma^*\tyUnit} = \tySem{\tyUnit}$, as required.
    \item[Case \TirName{TyPrim}] Since the index-erasure semantics
      ignores index expressions:
      $\tySem{\sigma^*\tyPrim{X}{e_1,...,e_n}} =
      \tySem{\tyPrim{X}{\sigma^*e_1,...,\sigma^*e_n}} = \tyPrimSem{X}
      = \tySem{\tyPrim{X}{e_1,...,e_n}}$.
    \item[Case \TirName{TyArr}] We have $A = A_1 \tyArr A_2$, and by
      the induction hypothesis, we know that $\tySem{\sigma^*A_1} =
      \tySem{A_1}$ and $\tySem{\sigma^*B_1} = \tySem{B_1}$. Thus, by
      the definition of substitution on arrow types, we have
      $\tySem{\sigma^*(A_1 \tyArr A_2)} = \tySem{\sigma^*A_1 \tyArr
        \sigma^*A_2} = \tySem{\sigma^*A_1} \to \tySem{\sigma^*A_2} =
      \tySem{A_1} \to \tySem{A_2} = \tySem{A_1 \tyArr A_2}$, as
      required.
    \item[Case \TirName{TyProd}] We have $A = A_1 \tyProduct A_2$, and
      by the induction hypothesis, we know that $\tySem{\sigma^*A_1} =
      \tySem{A_1}$ and $\tySem{\sigma^*A_2} = \tySem{A_2}$. Thus, by
      the definition of substitution on product types, we have
      $\tySem{\sigma^*(A_1 \tyProduct A_2)} = \tySem{\sigma^*A_1
        \tyProduct \sigma^*A_2} = \tySem{\sigma^*A_1} \times
      \tySem{\sigma^*A_2} = \tySem{A_1} \times \tySem{A_2} =
      \tySem{A_1 \tyProduct A_2}$, as required.
    \item[Case \TirName{TySum}] We have $A = A_1 + A_2$, and by the
      induction hypothesis, we know that $\tySem{\sigma^*A_1} =
      \tySem{A_1}$ and $\tySem{\sigma^*A_2} = \tySem{A_2}$. Thus, by
      the definition of substitution on sum types, we have
      $\tySem{\sigma^*(A_1 + A_2)} = \tySem{\sigma^*A_1 + \sigma^*A_2}
      = \tySem{\sigma^*A_1} + \tySem{\sigma^*A_2} = \tySem{A_1} +
      \tySem{A_2} = \tySem{A_1 + A_2}$, as required.
    \item[Case \TirName{TyForall}] We have $A = \forall
      i\mathord:s.A'$, and by the induction hypothesis we know that,
      for all $\sigma'$, $\tySem{\sigma'^*A'} =
      \tySem{A'}$. Therefore, from the definition of substitution for
      $\forall$-types, we have $\tySem{\sigma^*\forall i\mathord:s.A'}
      = \tySem{\forall i\mathord:s.\sigma_s^{*}A'} =
      \tySem{\sigma_s^{*}A'} = \tySem{A'} = \tySem{\forall
        i\mathord:s.A'}$, where we have relied on the fact that the
      index-erasure semantics of types ignores the index
      quantification.
    \end{description}
  \end{enumerate}
\end{proof}

% FIXME: make this look better
\begin{lemma}[\lemref{lem:tyeqsubst-relational}]
  \begin{enumerate}
  \item If $\Delta \vdash A \equiv B \isType$, then for all $\rho \in
    \relEnv{E}(\Delta)$, $\rsem{A}{\relEnv{E}}{\rho} =
    \rsem{B}{\relEnv{E}}{\rho}$;
  \item If $\Delta' \vdash A \isType$ and $\sigma : \Delta \Rightarrow
    \Delta'$, then for all $\rho \in \relEnv{E}(\Delta)$,
    $\rsem{\sigma^*A}{\relEnv{E}}\rho = \rsem{A}{\relEnv{E}}(\rho
    \circ \sigma)$.
  \end{enumerate}
\end{lemma}
\begin{proof}
  \begin{enumerate}
  \item By induction on the derivation of $\Delta \vdash A \equiv B
    \isType$.
    \begin{description}
    \item[Case \TirName{TyEqUnit}] In this case $A = B = \tyUnit$, so
      the statement is trivially statisfied.
    \item[Case \TirName{TyEqPrim}] In this case we have $A =
      \tyPrim{X}{e_1,...,e_n}$ and $B = \tyPrim{X}{e'_1,...,e'_n}$,
      with $\Delta \vdash e_j \equiv e'_j : s_j$. By ou requirement
      that relation environments preserve equality of simultaneous
      substitutions we have that $\rho_{\tyPrimNm{X}}(e_1,...,e_n) =
      \rho_{\tyPrimNm{X}}(e'_1,...,e'_n)$ and hence
      $\rsem{\tyPrim{X}{e_1,...,e_n}}{\relEnv{E}}\rho =
      \rsem{\tyPrim{X}{e'_1,...,e'_n}}{\relEnv{E}}\rho$.
    \item[Case \TirName{TyEqArr}] We have $A = A_1 \tyArr A_2$ and $B
      = B_1 \tyArr B_2$, with $\Delta \vdash A_1 \equiv B_1 \isType$
      and $\Delta \vdash A_2 \equiv B_2 \isType$. By the induction
      hypothesis, we know that $\rsem{A_1}{\relEnv{E}}\rho =
      \rsem{B_1}{\relEnv{E}}\rho$ and $\rsem{A_2}{\relEnv{E}}\rho =
      \rsem{B_2}{\relEnv{E}}\rho$. Thus we may reason as follows:
      $\rsem{A_1 \tyArr A_2}{\relEnv{E}}\rho =
      \rsem{A_1}{\relEnv{E}}\rho \relArrow \rsem{A_2}{\relEnv{E}}\rho
      = \rsem{B_1}{\relEnv{E}}\rho \relArrow
      \rsem{B_2}{\relEnv{E}}\rho = \rsem{B_1 \tyArr
        B_2}{\relEnv{E}}\rho$, as required.
    \item[Case \TirName{TyEqProd}] We have $A = A_1 \tyProduct A_2$
      and $B = B_1 \tyProduct B_2$, with $\Delta \vdash A_1 \equiv B_1
      \isType$ and $\Delta \vdash A_2 \equiv B_2 \isType$. By the
      induction hypothesis, we know that $\rsem{A_1}{\relEnv{E}}\rho =
      \rsem{B_1}{\relEnv{E}}\rho$ and $\rsem{A_2}{\relEnv{E}}\rho =
      \rsem{B_2}{\relEnv{E}}\rho$. Therefore, we can reason as
      follows: $\rsem{A_1 \tyProduct A_2}{\relEnv{E}}\rho =
      \rsem{A_1}{\relEnv{E}}\rho \relTimes \rsem{A_2}{\relEnv{E}}\rho
      = \rsem{B_1}{\relEnv{E}}\rho \relTimes
      \rsem{B_2}{\relEnv{E}}\rho = \rsem{B_1 \tyProduct
        B_2}{\relEnv{E}}\rho$, as required.
    \item[Case \TirName{TyEqSum}] We have $A = A_1 + A_2$ and $B = B_1
      + B_2$, with $\Delta \vdash A_1 \equiv B_1 \isType$ and $\Delta
      \vdash A_2 \equiv B_2 \isType$. By the induction hypothesis, we
      know that $\rsem{A_1}{\relEnv{E}}\rho =
      \rsem{B_1}{\relEnv{E}}\rho$ and $\rsem{A_2}{\relEnv{E}}\rho =
      \rsem{B_2}{\relEnv{E}}\rho$. Therefore, we can reason as
      follows: $\rsem{A_1 + A_2}{\relEnv{E}}\rho =
      \rsem{A_1}{\relEnv{E}}\rho \relSum \rsem{A_2}{\relEnv{E}}\rho =
      \rsem{B_1}{\relEnv{E}}\rho \relSum \rsem{B_2}{\relEnv{E}}\rho =
      \rsem{B_1 + B_2}{\relEnv{E}}\rho$, as required.
    \item[Case \TirName{TyEqForall}] We have $A = \forall
      i\mathord:s. A'$ and $B = \forall i\mathord:s.B'$, with $\Delta,
      i : s \vdash A' \equiv B' \isType$. By the induction hypothesis,
      we know that for all $\rho'$, $\rsem{A'}{\relEnv{E}}\rho' =
      \rsem{B'}\rho'$. We reason as follows:
      \begin{eqnarray*}
        &    & (x_1,x_2) \in \rsem{\forall i\mathord:s. A'}{\relEnv{E}}\rho \\
        &\iff& \forall \rho' \in \extends{\rho}{i:s}.\ (x_1,x_2) \in \rsem{A'}{\relEnv{E}}\rho' \\
        &\iff& \forall \rho' \in \extends{\rho}{i:s}.\ (x_1,x_2) \in \rsem{B'}{\relEnv{E}}\rho' \\
        &\iff& (x_1,x_2) \in \rsem{\forall i\mathord:s. B'}{\relEnv{E}}\rho
      \end{eqnarray*}
      Thus, by extensionality, we have $\rsem{\forall
        i\mathord:s.A'}\rho \equiv \rsem{\forall
        i\mathord:s.B'}{\relEnv{E}}\rho$, as required.
    \end{description}
  \item By induction on the derivation of $\Delta \vdash A \isType$. We
    analyse each case in turn:
    \begin{description}
    \item[Case \TirName{TyUnit}] Directly from the definition of
      substitution on types of the form $\tyUnit$, and the fact that
      $\rsem{\tyUnit}{\relEnv{E}}\rho_1 =
      \rsem{\tyUnit}{\relEnv{E}}\rho_2$ for any pair $\rho_1,\rho_2$
      of relation environments, we have
      $\rsem{\sigma^*\tyUnit}{\relEnv{E}}\rho =
      \rsem{\tyUnit}{\relEnv{E}}{(\rho \circ \sigma^*)}$, as required.
    \item[Case \TirName{TyPrim}] We have $A =
      \tyPrim{X}{e_1,...,e_n}$, therefore
      $\rsem{\sigma^*A}{\relEnv{E}}\rho =
      \rsem{\sigma^*\tyPrim{X}{e_1,...,e_n}}{\relEnv{E}}\rho =
      \rsem{\tyPrim{X}{\sigma^*e_1,...,\sigma^*e_n}}{\relEnv{E}}\rho =
      \rho_{\tyPrimNm{X}}(\sigma^*e_1,...,\sigma^*e_n) =
      \rsem{\tyPrim{X}{e_1,...,e_n}}{\relEnv{E}}{(\rho \circ
        \sigma^*)}$, as required.
    \item[Case \TirName{TyArr}] In this case, $A = A_1 \tyArr A_2$ and
      by the induction hypothesis, we know that
      $\rsem{\sigma^*A_1}{\relEnv{E}}\rho =
      \rsem{A_1}{\relEnv{E}}{(\rho \circ \sigma^*)}$ and
      $\rsem{\sigma^*A_2}{\relEnv{E}}\rho =
      \rsem{A_2}{\relEnv{E}}{(\rho \circ \sigma^*)}$. Accordingly, we
      reason as follows: $\rsem{\sigma^*(A_1 \tyArr
        A_2)}{\relEnv{E}}\rho = \rsem{\sigma^*A_1 \tyArr
        \sigma^*A_2}{\relEnv{E}}\rho =
      \rsem{\sigma^*A_1}{\relEnv{E}}\rho \relArrow
      \rsem{\sigma^*A_2}{\relEnv{E}}\rho =
      \rsem{A_1}{\relEnv{E}}{(\rho \circ \sigma^*)} \relArrow
      \rsem{A_2}{\relEnv{E}}{(\rho \circ \sigma^*)} = \rsem{A_1 \tyArr
        A_2}{\relEnv{E}}{(\rho \circ \sigma^*)}$, as required.
    \item[Case \TirName{TyProd}] In this case, $A = A_1 \tyProduct
      A_2$ and by the induction hypothesis, we know that
      $\rsem{\sigma^*A_1}{\relEnv{E}}\rho =
      \rsem{A_1}{\relEnv{E}}{(\rho \circ \sigma^*)}$ and
      $\rsem{\sigma^*A_2}{\relEnv{E}}\rho =
      \rsem{A_2}{\relEnv{E}}{(\rho \circ \sigma^*)}$. Accordingly, we
      reason as follows: $\rsem{\sigma^*(A_1 \tyProduct
        A_2)}{\relEnv{E}}\rho = \rsem{\sigma^*A_1 \tyProduct
        \sigma^*A_2}{\relEnv{E}}\rho =
      \rsem{\sigma^*A_1}{\relEnv{E}}\rho \relTimes
      \rsem{\sigma^*A_2}{\relEnv{E}}\rho =
      \rsem{A_1}{\relEnv{E}}{(\rho \circ \sigma^*)} \relTimes
      \rsem{A_2}{\relEnv{E}}{(\rho \circ \sigma^*)} = \rsem{A_1
        \tyProduct A_2}{\relEnv{E}}{(\rho \circ \sigma^*)}$, as
      required.
    \item[Case \TirName{TySum}] In this case, $A = A_1 + A_2$ and by
      the induction hypothesis, we know that
      $\rsem{\sigma^*A_1}{\relEnv{E}}\rho =
      \rsem{A_1}{\relEnv{E}}{(\rho \circ \sigma^*)}$ and
      $\rsem{\sigma^*A_2}{\relEnv{E}}\rho =
      \rsem{A_2}{\relEnv{E}}{(\rho \circ \sigma^*)}$. Accordingly, we
      reason as follows: $\rsem{\sigma^*(A_1 + A_2)}{\relEnv{E}}\rho =
      \rsem{\sigma^*A_1 + \sigma^*A_2}{\relEnv{E}}\rho =
      \rsem{\sigma^*A_1}{\relEnv{E}}\rho \relSum
      \rsem{\sigma^*A_2}{\relEnv{E}}\rho =
      \rsem{A_1}{\relEnv{E}}{(\rho \circ \sigma^*)} \relSum
      \rsem{A_2}{\relEnv{E}}{(\rho \circ \sigma^*)} = \rsem{A_1 +
        A_2}{\relEnv{E}}{(\rho \circ \sigma^*)}$, as required.
    \item[Case \TirName{TyForall}] We have $A = \forall
      i\mathord:s.A'$. We prove the required equation by demonstrating
      two inclusions. From left-to-right, we know that
      \begin{equation}
        \label{eq:tysubst-rel-forall1}
        (x_1,x_2) \in \rsem{\sigma^*\forall i\mathord:s. A'}{\relEnv{E}}\rho
      \end{equation}
      and we must show that $(x_1, x_2) \in \rsem{\forall
        i\mathord:s. A'}{\relEnv{E}}{(\rho \circ \sigma^*)}$. From
      (\ref{eq:tysubst-rel-forall1}) and the definition of
      substitution, we know that
      \begin{displaymath}
        \forall \rho' \in \extends{\rho}{i:s}.\ (x_1,x_2) \in \rsem{\sigma_s^*A'}{\relEnv{E}}\rho'
      \end{displaymath}
      By the induction hypothesis, we can deduce that
      \begin{equation}
        \label{eq:tysubst-rel-forall2}
        \forall \rho' \in \extends{\rho}{i:s}.\ (x_1,x_2) \in \rsem{A'}{\relEnv{E}}{(\rho' \circ \sigma_s^{*})}
      \end{equation}
      To show the required inclusion, we must show that for all
      $\rho_1 \in \extends{\rho \circ \sigma^*}{i:s}$, it is the case
      that $(x_1,x_2) \in \rsem{A'}{\relEnv{E}}{\rho_1}$. We now make
      use of the pushout property of our family $\relEnv{E}$ of
      relation environments: we have a $\rho \in \relEnv{E}(\Delta)$
      and $\rho_1 \in \relEnv{E}(\Delta, i:s)$ such that $\rho_1 \circ
      \pi_{i:s} = \rho \circ \sigma^*$ (by the assumption that $\rho_1
      \in \extends{\rho \circ \sigma^*}{i:s}$), so we can obtain a
      $\rho' \in \relEnv{E}(\Delta',i:s)$ such that $\rho' \circ
      \pi_{i:s} = \rho$ (so $\rho' \in \extends{\rho}{i:s}$), and
      $\rho' \circ \sigma^* = \rho_1$. Therefore we use
      (\ref{eq:tysubst-rel-forall2}) to deduce that $(x_1,x_2) \in
      \rsem{A'}{\relEnv{E}}{\rho_1}$, and the inclusion from
      left-to-right is shown.

      From right-to-left, we must now show
      (\ref{eq:tysubst-rel-forall2}) under the assumption that
      \begin{equation}
        \label{eq:tysubst-rel-forall3}
        \forall \rho_1 \in \extends{\rho \circ \sigma^*}{i:s}. (x_1,x_2) \in \rsem{A'}{\relEnv{E}}{\rho_1}.
      \end{equation}
      Given $\rho' \in \extends{\rho}{i:s}$, we let $\rho_1 = \rho'
      \circ \sigma^*$. Now, $\rho_1 \circ \pi_{i:s} = \rho' \circ
      \sigma^* \circ \pi_{i:s} = \rho' \circ \pi_{i:s} \circ
      \sigma_s^{*} = \rho \circ \sigma_s^{*}$. Thus $\rho_1 \in
      \extends{\rho \circ \sigma^*}{i:s}$ and we may use
      (\ref{eq:tysubst-rel-forall3}) to deduce that $(x_1,x_2) \in
      \rsem{A'}{\relEnv{E}}{(\rho' \circ \sigma_s^{*})}$, as required.
    \end{description}
    The second part of the lemma statement follows directly by
    induction on the derivation of $\Delta \vdash \Gamma \isCtxt$ and
    the first part. The step case of the induction is very similar to
    the \TirName{TyProd} case above.
  \end{enumerate}
\end{proof}
